src/PermProgAuto.v
@@ -32,44 +32,44 @@ Ltac inv_exec'' H :=
 
 Ltac inv_exec' :=
   match goal with
-  | [ H: exec _ _ _ _ _ (Ret _) _ _ |- _ ] =>
+  | [ H: exec _ _ _ _ (Ret _) _ _ |- _ ] =>
     inv_exec'' H
-  | [ H: exec _ _ _ _ _ (Read _) _ _ |- _ ] =>
+  | [ H: exec _ _ _ _ (Read _) _ _ |- _ ] =>
     inv_exec'' H
-  | [ H: exec _ _ _ _ _ (Write _ _) _ _ |- _ ] =>
+  | [ H: exec _ _ _ _ (Write _ _) _ _ |- _ ] =>
     inv_exec'' H
-  | [ H: exec _ _ _ _ _ (Seal _ _) _ _ |- _ ] =>
+  | [ H: exec _ _ _ _ (Seal _ _) _ _ |- _ ] =>
     inv_exec'' H
-  | [ H: exec _ _ _ _ _ (Unseal _) _ _ |- _ ] =>
+  | [ H: exec _ _ _ _ (Unseal _) _ _ |- _ ] =>
     inv_exec'' H
-  | [ H: exec _ _ _ _ _ Sync _ _ |- _ ] =>
+  | [ H: exec _ _ _ _ Sync _ _ |- _ ] =>
     inv_exec'' H
-  | [ H: exec _ _ _ _ _ (Hash _) _ _ |- _ ] =>
+  | [ H: exec _ _ _ _ (Hash _) _ _ |- _ ] =>
     inv_exec'' H
-  | [ H: exec _ _ _ _ _ (Hash2 _ _) _ _ |- _ ] =>
+  | [ H: exec _ _ _ _ (Hash2 _ _) _ _ |- _ ] =>
     inv_exec'' H
-  | [ H: exec _ _ _ _ _ (Auth _) _ _ |- _ ] =>
+  | [ H: exec _ _ _ _ (Auth _) _ _ |- _ ] =>
     inv_exec'' H
   end.
 
 Lemma bind_sep:
-  forall T T' pr (p1: prog T) (p2: T -> prog T') d bm hm (ret: result) tr tr',
-    exec pr tr d bm hm (Bind p1 p2) ret tr' ->
+  forall T T' pr (p1: prog T) (p2: T -> prog T') d bm hm (ret: result) tr',
+    exec pr d bm hm (Bind p1 p2) ret tr' ->
     match ret with
     | Finished _ _ _ _ =>
-    (exists tr1 r1 d1 bm1 hm1,
-       exec pr tr d bm hm p1 (Finished d1 bm1 hm1 r1) tr1 /\
-       exec pr tr1 d1 bm1 hm1 (p2 r1) ret tr')
+    (exists tr1 tr2 r1 d1 bm1 hm1,
+       exec pr d bm hm p1 (Finished d1 bm1 hm1 r1) tr1 /\
+       exec pr d1 bm1 hm1 (p2 r1) ret tr2 /\ tr' = tr2 ++ tr1)
   | Crashed d' bm' hm' =>
-    (exec pr tr d bm hm p1 (Crashed d' bm' hm') tr' \/
-     (exists tr1 r1 d1 bm1 hm1,
-        exec pr tr d bm hm p1 (Finished d1 bm1 hm1 r1) tr1 /\
-        exec pr tr1 d1 bm1 hm1 (p2 r1) ret tr'))
+    (exec pr d bm hm p1 (Crashed d' bm' hm') tr' \/
+     (exists tr1 tr2 r1 d1 bm1 hm1,
+        exec pr d bm hm p1 (Finished d1 bm1 hm1 r1) tr1 /\
+        exec pr d1 bm1 hm1 (p2 r1) ret tr2 /\ tr' = tr2 ++ tr1))
    | Failed d' bm' hm' =>
-    (exec pr tr d bm hm p1 (Failed d' bm' hm') tr' \/
-     (exists tr1 r1 d1 bm1 hm1,
-        exec pr tr d bm hm p1 (Finished d1 bm1 hm1 r1) tr1 /\
-        exec pr tr1 d1 bm1 hm1 (p2 r1) ret tr'))
+    (exec pr d bm hm p1 (Failed d' bm' hm') tr' \/
+     (exists tr1 tr2 r1 d1 bm1 hm1,
+        exec pr d bm hm p1 (Finished d1 bm1 hm1 r1) tr1 /\
+        exec pr d1 bm1 hm1 (p2 r1) ret tr2 /\ tr' = tr2 ++ tr1))
     end.
 Proof.
   intros.
@@ -148,6 +148,6 @@ Ltac split_ors:=
 
 Ltac inv_exec_perm :=
   match goal with
-  |[H : exec _ _ _ _ _ (Bind _ _) _ _ |- _ ] => apply bind_sep in H; repeat cleanup
-  |[H : exec _ _ _ _ _ _ _ _ |- _ ] => inv_exec'
+  |[H : exec _ _ _ _ (Bind _ _) _ _ |- _ ] => apply bind_sep in H; repeat cleanup
+  |[H : exec _ _ _ _ _ _ _ |- _ ] => inv_exec'
   end.
