src/PermSec.v
@@ -22,30 +22,6 @@ Fixpoint trace_secure pr tr :=
           trace_secure pr t
   end.
 
-(* adding state allows simpler bind *)
-(* Not in use anymore *)
-Fixpoint permission_secure {T} d bm hm pr (p: prog T) :=
-match p with
-| Seal t _ => can_access pr t
-| Unseal h => forall tb, bm h = Some tb -> can_access pr (fst tb)
-| Bind p1 p2 => permission_secure d bm hm pr p1 /\
-                (forall d' bm' hm' r tr tr',
-                exec pr tr d bm hm p1 (Finished d' bm' hm' r) tr' ->
-                permission_secure d' bm' hm' pr (p2 r))
-| _ => True
-end.
-
-Lemma trace_app:
-  forall  T (p: prog T) pr d bm hm tr r tr',
-    exec pr tr d bm hm p r tr' ->
-    exists tr'', tr' = tr''++tr.
-Proof.
-  induction 1; intuition; repeat inv_exec_perm; try solve [exists nil; eauto].
-  exists (Sea t::nil); eauto.
-  exists (Uns (fst tb)::nil); eauto.
-  cleanup; eexists; rewrite <- app_assoc; eauto.
-Qed.
-
 Lemma trace_secure_app:
   forall pr tr1 tr2,
     trace_secure pr tr1 ->
